Done separating ilist from the actual message format.

src/Narcissus/Examples/PermutationOpt.v
@@ -10,11 +10,11 @@ Require Import Coq.Sorting.Permutation.
 Require Import Fiat.Narcissus.Automation.Invertible.
 
 Require Import
-        Fiat.Common.ilist
-        Fiat.Common.SumType.
+  Fiat.Common.ilist
+  Fiat.Common.SumType.
 
 Require Import
-        Coq.Logic.FinFun.
+  Coq.Logic.FinFun.
 Import Fin2Restrict.
 
 Set Warnings "-local-declaration".
@@ -66,11 +66,11 @@ Module Permutation.
 
   Ltac new_encoder_rules ::=
     eapply Permutation_Encoder_Correct;
-      [| unfold Vector.nth; repeat constructor | |IndexedSumType.split_iterate ]; simpl;
-      eauto with resilience.
+    [| unfold Vector.nth; repeat constructor | |IndexedSumType.split_iterate ]; simpl;
+    eauto with resilience.
   Definition inv (msg: message):= True.
   
-  Let enc_dec : EncoderDecoderPair (permutation_Format myProjections myFinFormat myFormats ++ empty_Format) inv.
+  Let enc_dec : EncoderDecoderPair (permutation_Format myProjections myFinFormat myFormats) inv.
   Proof.
     unfold myFinFormat.
     (* derive_encoder_decoder_pair. *)
@@ -87,766 +87,636 @@ Module Permutation.
                       ltac:(fun invariants' =>
                               Vector_of_evar 2 (Ensembles.Ensemble (CacheDecode -> Prop))
                                 ltac:(fun cache_invariants' =>
-                                        eapply Permutation_decoder with
+                                        eapply Permutation_decoder_Correct with
                                         (cache_invariants := cache_invariants')
                                         (invariants:= invariants')
                                         (decoders:= decoders')
-                           )));
-    try solve[apply_rules]; cycle 1.
-    * split. 2: split. 
-      all: simpl; intros.
-      apply_rules.
-      apply_rules.
-      constructor.
-    * intros ????.
-      repeat (split; auto).
-    * Transparent cache_inv_Property.
-      unfold cache_inv_Property in *; repeat split;
-        unfold Vector.nth; simpl in *; auto.
-      shelve.
-      shelve.
-    * (* extract_view *)
-      (* ExtractSource *)
-      
-      Definition decidesOpt {a} (op: option a) (predicate: a -> Prop):=
-        Ifopt op as s Then predicate s Else forall s, ~ predicate s.
+                 )));
+                                           try solve[apply_rules]; cycle 1.
+        * split. 2: split. 
+          all: simpl; intros.
+          apply_rules.
+          apply_rules.
+          constructor.
+        * intros ???.
+          repeat (split; auto).
+        * intros.
+          (* ExtractSource *)
+          eapply CorrectDecoderEmpty.
+          -- (* build_fully_determined_type *)
+            unfold Heading.Domain, Tuple.GetAttribute, Tuple.GetAttributeRaw,
+              Basics.compose in *; simpl in *.
+            
+            let a' := fresh in
+            intros a'; try destruct a'; destruct_conjs.
 
-      
-      Definition decidesOptBool {a} (op: option a) (b: a -> bool) (predicate: a -> Prop):=
-        Ifopt op as s Then (decides (b s) (predicate s)) Else forall s, ~ predicate s.
+            unfold Heading.Domain, Tuple.GetAttribute, Tuple.GetAttributeRaw in *;
+              simpl in *; intros; decompose_source_predicate. subst_projections.
+            simpl in *.
 
-      Definition filter_decode {S B} (op:option S): DecodeM (S * B) B:=
-        (fun t' ctxD =>
-           match op with
-           | Some s => Some (s, t', ctxD)
-           | _ =>  None
-           end).
+            Class ConditionallyInvertibleTwo {A0 A1 B : Type} (F: A0 -> A1 -> B)(P : A0 -> A1 -> Prop)
+              (F0: B -> A0)(F1: B -> A1) :=
+              { CInvTwoRoundTrip0 : forall a0 a1, P a0 a1 -> F0 (F a0 a1) = a0;
+                CInvTwoRoundTrip1 : forall a0 a1, P a0 a1 -> F1 (F a0 a1) = a1}.
+            
+            (* This lemma restates the invertible condition as a manipulation of
+           equations.   *)
+            Lemma CInvTwo_equation :
+              forall A0 A1 B F P F0 F1 {CInv: @ConditionallyInvertibleTwo A0 A1 B F P F0 F1},
+              forall a0 a1 b, P a0 a1 -> F a0 a1 = b -> a0 = F0 b /\ a1 = F1 b.
+            Proof. intros * ? *  ? HH. rewrite <- HH.
+                   rewrite CInvTwoRoundTrip0; auto.
+                   rewrite CInvTwoRoundTrip1; auto. Qed.
+            
+            Ltac subst_invertible_functions_two :=
+              match goal with
+              | H:?f ?x ?y = _
+                |- _ =>
+                  eapply (CInvTwo_equation _ _ _ f) in H;
+                  idtac H;
+                  [ destruct H | now typeclasses eauto | now simpl in *; eauto ]; 
+                  try subst x
+              end.
 
-      
-      Definition filter_decode_bool {S B} (op:option S) (b:S -> bool) : DecodeM (S * B) B:=
-        (fun t' ctxD =>
-           match op with
-           | Some s => if (b s) then Some (s, t', ctxD) else None
-           | _ =>  None
-           end).
+            Instance icons_invert {A B} {a:A} {n:nat} l  :
+              ConditionallyInvertibleTwo (@icons _ B a n l) (fun _ _ => True) (ilist_hd') (ilist_tl').
+            Proof.
+              constructor; reflexivity.
+            Qed.
+            
+            repeat subst_invertible_functions_two.
+            reflexivity.
+          -- simpl.
+             unfold inv.
+             eapply decides_and.
+             apply decides_True'.
+             simpl.
+             unfold IsProj, iapp; simpl.
+             Print HintDb decide_data_invariant_db.
+             
+             Lemma decides_ilist_projections':
+               forall {a n l} ils x y b_x b_y ,
+                 decides b_x (x = prim_fst ils) -> 
+                 decides b_y (y = prim_snd ils) ->
+                 decides (b_x && b_y)
+                   (@icons Type id a n l x y = ils).
+             Proof.
+               simpl.
+               intros.
+               eapply decides_mor_Proper; [reflexivity| | ]; cycle 1.
+               eapply decides_and; eauto.
+               destruct ils; simpl in *.
+               split; intros H1.
+               - inversion H1; auto.
+               - destruct H1; subst; eauto.
+             Qed.
+             Lemma decides_ilist_projections0:
+               forall {a} ils x y b_x b_y ,
+                 decides b_x (x = prim_fst ils) -> 
+                 decides b_y (y = prim_snd ils) ->
+                 decides (b_x && b_y)
+                   (@icons Type id a 0 (Vector.nil _) x y = ils).
+             Proof.
+               intros.
+               eapply decides_ilist_projections'; eauto.
+             Qed.
+             
+             Lemma decides_ilist_projections:
+               forall {a n l} (ils: ilist(B:=id) (Vector.cons Type a n l)) x y b_x b_y ,
+                 decides b_x (x = prim_fst ils) -> 
+                 decides b_y (y = prim_snd ils) ->
+                 decides (b_x && b_y)
+                   (icons x y = ils).
+             Proof.
+               simpl; intros. eapply decides_ilist_projections'; eauto.
+             Qed.
 
+             Global Hint Resolve decides_ilist_projections : HintDb decide_data_invariant_db.
+             eauto with HintDb decide_data_invariant_db.
+             
+             Ltac blah:= match goal with
+                         | |- decides _ (_ = ?v) =>
+                             eapply (decides_ilist_projections v)
+                         | |- decides _ (_ = ?v) =>
+                             eapply (decides_ilist_projections0 v)
+                         | |- decides _ (_ = ?v) =>
+                             eapply (decides_ilist_projections' v)
+                         end.
+             repeat first[blah | apply decides_eq_refl].
 
-      (** *Comment this one*)
-      (* eapply CorrectDecoderEmpty. *)
-      
-      Corollary CorrectDecoderEmptyOptBool {S T}
-        : forall (monoid : Monoid T)
-            (Source_Predicate : S -> Prop)
-            (decode_inv : CacheDecode -> Prop)
-            (op : option S) (b: S-> bool),
-          (forall s', Ifopt op as s Then Source_Predicate s' -> s' = s Else True) ->
-          decidesOptBool op b Source_Predicate 
-          -> CorrectDecoder
-              monoid
-              Source_Predicate
-              Source_Predicate
-              eq
-              empty_Format
-              (filter_decode_bool op b)
-              decode_inv
-              empty_Format.
-        Admitted.
-        
-      Corollary CorrectDecoderEmptyOpt {S T}
-        : forall (monoid : Monoid T)
-            (Source_Predicate : S -> Prop)
-            (decode_inv : CacheDecode -> Prop)
-            (op : option S),
-          (forall s', Ifopt op as s Then Source_Predicate s' -> s' = s Else True) ->
-          decidesOpt op Source_Predicate 
-          -> CorrectDecoder
-              monoid
-              Source_Predicate
-              Source_Predicate
-              eq
-              empty_Format
-              (filter_decode op)
-              decode_inv
-              empty_Format.
-      Proof.
-        intros.
-        destruct op.
-        - eapply ExtractViewFrom; eauto; unfold empty_Format; eauto.
-        - Transparent CorrectDecoder.
-          unfold CorrectDecoder, empty_Format; split. intros.
-          + elimtype False; eapply H0. eauto.
-          + discriminate.
-      Qed.
-      
-      Fixpoint sortType {m} {types : Vector.t Type m}
-        (ls: list (SumType types)): option (ilist (B:=id) types).
-      Admitted.
+             Ltac match_inside_prim_snd x k:=
+               match x with
+               | prim_snd ?x' => match_inside_prim_snd x' k
+               | ?x' => k x
+               end.
+             Ltac destruct_ilist x:=
+               match type of x with
+               | (ilist []) => destruct x
+               | _ => let y:= fresh "x" in
+                     destruct x as [? y];
+                     destruct_ilist y 
+               end.
+             
+             match goal with
+               |- decides _ (inil = ?x) =>
+                 match_inside_prim_snd x
+                   ltac:(destruct_ilist)
+             end; simpl.
+             apply decides_eq_refl.
+             
+             
+        * Transparent cache_inv_Property.
+          unfold cache_inv_Property in *; simpl in *; repeat split;
+            unfold Vector.nth; simpl in *; auto.
+          instantiate(2:= constant True); constructor.
+          
+      + cbv beta; synthesize_cache_invariant.
+      + cbv beta; unfold decode_nat, sequence_Decode;
+          optimize_decoder_impl.
+      + cbv beta; align_decoders.
+        ltac:(cbv beta; unfold decode_nat, sequence_Decode;
+              optimize_decoder_impl) ltac:(cbv beta; align_decoders)
 
-      
-      
-      simpl; intros.
-      eapply CorrectDecoderEmptyOpt.
-      
-      -- unfold Heading.Domain, Tuple.GetAttribute, Tuple.GetAttributeRaw,
-           Basics.compose in *; simpl in *.
-         let a' := fresh in
-         intros a'; try destruct a'.
-         match goal with
-           |- context [If_Opt_Then_Else ?x _ _] =>
-             destruct x as [XX|] eqn:HeqXX; simpl; auto
-         end.
-         unfold inv; simpl; intros [].
-         simpl in H3.
-         clear H1.
-         assert (HH:forall  s s', iapp myProjections s = iapp myProjections s' -> s = s'); cycle 1.
-         eapply HH; simpl.
-
-         Definition messageFromIlist 
-           (ls: ilist(B:=id) types) : option message.
-         Proof.
-           unfold types in *.
-           destruct ls as [T0 ls].
-           destruct ls as [T1 _].
-           unfold id in *.
-           left; constructor; eauto.
-         Defined. (*Can't be stated for a generic `message`. Prove in Ltac*)
-         
-         Fixpoint messageFromlist
-           (ls: list (SumType types)): option message :=
-           match sortType ls with
-           | Some i => messageFromIlist i
-           | None => None
-           end.
-           
-         instantiate(1:=messageFromlist v1) in HeqXX.
-         
-         
-         
-         (* What needs to be done:
-            Rewrite the format to be a format of ilist.
-            Then we can compose it to make it a format of S (e.g. `message`)
-
-
-          *)
-         
-         admit. (* Cant be stated as a lemma prove in Ltac. *)
-         
-         admit. (*Projections must be injective. Easy Ltac proof*) 
-         
-         
-
-     
-      -- match goal with
-           |- decidesOptBool ?x _ _ => destruct x eqn:HHx; simpl
-         end.
-         ++ eapply decides_and.
-            ** eapply decides_True'.
-            ** instantiate(1:= true).
-            admit.
-         ++ intros ? [_ ?].
-         
-         
-         
-        Lemma decidesOpt_and:
-           forall {B B'}
-             (ob : option B)(ob' : option B')
-             (P : B -> Prop)
-             (Q : B' -> Prop),
-             decidesOpt ob P ->
-             decidesOpt ob' Q ->
-             decidesOpt (match (ob, ob') with
-                      | (Some b, Some b') => Some (b, b')
-                      | _ => None
-                         end) (fun bb' => P (fst bb') /\ Q (snd bb')).
-         Admitted.
-
-         
-         
+                                            Ltac apply_new_combinator_rule ::=
+          eapply Permutation_decoder.
+        synthesize_aligned_decoder.
 
 
-        Lemma decidesOpt_and:
-           forall {B B'}
-             (ob : option B)(ob' : option B')
-             (P : B -> Prop)
-             (Q : B' -> Prop),
-             decidesOpt ob P ->
-             decidesOpt ob' Q ->
-             decidesOpt (match (ob, ob') with
-                      | (Some b, Some b') => Some (b, b')
-                      | _ => None
-                         end) (fun bb' => P (fst bb') /\ Q (snd bb')).
-         Admitted.
-          Lemma decidesOpt_and_r':
-           forall {B}
-             (ob : option B)(b' : bool )
-             (P : B -> Prop)
-             (Q : Prop),
-             decidesOpt ob P ->
-             decides b' Q ->
-             decidesOpt (if b' then ob else None) (fun ob => P ob /\ Q ).
-         Admitted. 
-         Lemma decidesOpt_and1:
-           forall {B}
-             (ob: option B)
-             (P : B -> Prop)
-             (Q : B -> Prop),
-             decidesOpt ob P ->
-             decidesOpt ob Q ->
-             decidesOpt ob (fun bb' => P bb' /\ Q bb').
-         Admitted.
-         
-         Lemma decidesOpt_true:
-           forall {B}
-             (ob: option B),
-             decidesOpt ob (constant True).
-         Admitted.
-         
-         eapply decidesOpt_and.
-         eapply decidesOpt_true.
+        *)
+(*
 
-         
 
-         
-         
-         Lemma decidesOpt_permutation:
-           forall {B n} {types: Vector.t Type n}
-             (ob: option B) v1
-             (f: option (ilist(B:=id) types) -> option (message))
-             (projs: ilist(B:= fun T => message -> T) types),
-             decidesOpt (f (sortType v1))
-               (fun s : message => Permutation (to_list projs s) v1).
-         Admitted.
-         eapply decidesOpt_permutation.
-         
-         
-         
-         
-         
-         
-        build_fully_determined_type.
-        decide_data_invariant.
 
-        exact (sortType v1).
 
-      
-      (* Need to assume that all the values in v1 are of different
-         types!  That way we know we can construct a canonincal
-         element from it.  Otherwise, `s` might not exists (notice the
-         only thing in the environment of `s` is `v1`. *)
 
-      (* SOLUTION: Wrap the format in a checking format that filters things
-         that don't satisfy the predicate!*)
 
-      2:{ 
-      2:{ decide_data_invariant.
-      [ build_fully_determined_type |  ] ]
 
-      
-    
-    * simpl.
-      
-    
-        
-        ilist_of_evar (fun T => DecodeM (T * ByteString) ByteString) types
-          ltac:(fun decoders' => 
-                  eapply Permutation_decoder ()).
-        
-        eapply Permutation_decoder; try solve[apply_rules].
-        * simpl.
-          Transparent cache_inv_Property.
-          unfold cache_inv_Property; repeat split.
+
+
+
+
+
+
+
+
+
+
+
+
+
+
+
+
+
+
+
+
+
+
+
+
+
+
+
 
           
-        admit.
-        
-        
-        
-        eapply Permutation_decoder.
-        
-      + cbv beta; synthesize_cache_invariant.
-   ltac:(cbv beta; unfold decode_nat, sequence_Decode;
-          optimize_decoder_impl) ltac:(cbv beta; align_decoders)
-
-      Ltac apply_new_combinator_rule ::=
-        eapply Permutation_decoder.
-      synthesize_aligned_decoder.
-
-
-*)
-
-
-
-
-
-
-
-
-
-
-
-
-
-
-
-
-
-
-
-
-
-
-
-
-
-
-
-
-
-
-
-
-
-
-
-
-  
-  
-(** * Old  version. *)
-(* This version builds the format from scratch. Great for exploration.
+          
+          (** * Old  version. *)
+          (* This version builds the format from scratch. Great for exploration.
 
 TODO: DELETE when the rest is ready!
-*)
-  
-Module PermutationCodes2.  
-  Let types:= [word 8:Type; word 16:Type].
-
-  Let myTuple:= ituple types.
-
-  Definition formats : ilist (B := fun T => FormatM T ByteString) types
-    := {{ format_word; format_word }}.
-  
-  Let invariants := ilist_constant_T types.
-  Let view_fin {n} (f:Fin.t n):= f2n f < pow2 8.
-  Let invariant := (fun st : SumType types =>
-                      view_fin (SumType_index types st) /\ ith invariants (SumType_index types st) (SumType_proj types st)).
-
-  Definition lift_SumType (A:Type) {n:nat} {types:Vector.t Type n} :
-    SumType types -> SumType (Vector.cons Type A _ types):=
-    match types as typs return
-          SumType typs -> SumType (Vector.cons Type A _ typs) with
-    | Vector.nil =>
-        (* Impossible case: with an empty vector can't construct the SumType*)
-        fun elem => let X1 := match elem return A with
-                           end in X1
-    | Vector.cons a n typs' =>
-        fun elem => inr elem
-    end.
-      
-  Fixpoint to_list {n:nat} {S:Type} {types:Vector.t Type n}:
-    forall projections: ilist (B:= fun T => S -> T) types, 
-      S -> list (SumType types):=
-    match types as typs return
-          ilist (B:= fun T => S -> T) typs ->  
-          S -> list (SumType typs) with
-    | Vector.nil => fun _ _ => Datatypes.nil
-    | @Vector.cons _ a n' typs' =>
-        let typs:= Vector.cons Type a n' typs' in
-        fun projs S =>
-          (inj_SumType typs Fin.F1 (prim_fst projs S))
-            :: map (lift_SumType a) (to_list (prim_snd projs) S)
-    end.
-
-   Definition format_SumType_list
-              (m : nat) (types : Vector.t Type m)
-              (fin_format: FormatM (Fin.t m) ByteString)
-             (formats: ilist (B:= fun T => FormatM T ByteString) types):
-     FormatM (list (SumType types)) ByteString:=
-     format_list (format_IndexedSumType m types formats fin_format).
-
-  
-  Definition format_permutation_list
-              (m : nat) (types : Vector.t Type m)
-              (fin_format: FormatM (Fin.t m) ByteString)
-             (formats: ilist (B:= fun T => FormatM T ByteString) types):
-    FormatM (list (SumType types)) ByteString:=
-    Compose_Format (format_SumType_list m types fin_format formats)
-               (Permutation (A:=SumType types)).
-      
-    
-  
-  Definition format_through_list
-             S
-             (m : nat) (types : t Type m)
-             (projections: ilist (B:= fun T => S -> T) types)
-             (fin_format: FormatM (Fin.t m) ByteString)
-             (formats: ilist (B:= fun T => FormatM T ByteString) types):
-    FormatM S ByteString:=
-    format_permutation_list m types fin_format formats ◦ to_list projections.
-    
-  Record message := {
-      label : word 8
-    ; data : word 16                     
-    }.
-
-  Let myProjections: ilist (B:=fun T => _ -> T) types := {{ label ; data }}.
-  Let myTypes {n: nat} {types: Vector.t Type n} {B} (list: ilist (B:=B) types): Vector.t Type n:= types.
-  
-  Let myCodes: Vector.t (word 8) 2:= [[ natToWord _ 42; natToWord _ 73 ]].
-  Let myFinFormat:= (format_enum myCodes).
-  
-  Let myFormats: ilist (B := fun T => FormatM T ByteString) (myTypes myProjections) := {{ format_word; format_word }}.
-  
-  Let myFormat:= format_through_list message _ types myProjections myFinFormat myFormats.
-  
-  Let enc_dec : EncoderDecoderPair myFormat (constant True).
-  Proof.
-    (*unfold myFormat,format_through_list, format_permutation_list.*)
-    (* derive_encoder_decoder_pair. *)
-    econstructor.
-    - (* synthesize_aligned_encoder. *)
-      start_synthesizing_encoder.
-      normalize_encoder_format.
-      
-      align_encoder_step. (*splits emty*)
-      align_encoder_step. (* removes empty*)
-      (*eapply CorrectAlignedEncoderProjection.*)
-      align_encoder_step. (*projection*)
-      
-      unfold format_permutation_list.
-      match goal with
-        |- CorrectAlignedEncoder (Compose_Format ?X _) ?enc =>
-          cut (CorrectAlignedEncoder X enc) 
-      end.
-      + (*This should be trivial, since identity is a premutation*)
-        unfold format_SumType_list.
-        shelve.
-      + repeat align_encoder_step.
-    - (* synthesize_aligned_decoder. *)
-      start_synthesizing_decoder.
-      + Lemma EquivFormat_compose_projection {T S S' S''}
-              (format_S'' : FormatM S'' T)
-              (f : S -> S')
-              (r : S' -> S'' -> Prop)
-          : EquivFormat (Projection_Format (Compose_Format format_S'' r) f)
-                        (Compose_Format format_S'' (fun a b => r (f a) b)).
-        Proof.
-          unfold EquivFormat, refineEquiv, Projection_Format, Compose_Format, compose, Bind2; split;
-            intros ? ?.
-          - rewrite unfold_computes in *.
-            destruct_ex; split_and; eexists.
-            rewrite unfold_computes;  eauto.
-          - rewrite unfold_computes in *.
-            destruct_ex; split_and.
-            rewrite unfold_computes in H0.
-            destruct_ex; split_and.
-            eexists; intuition eauto.
-            subst; eauto.
-        Qed.
-
-        Ltac normalize_step BitStringT ::=
-          (first_debug
-             [ match goal with
-               | |- EquivFormat ?z ?x => is_evar z; apply EquivFormat_reflexive
-               end; idtac "1"
-             | eapply EquivFormat_trans; [ apply sequence_assoc |  ]
-               ; idtac "3"
-             | eapply EquivFormat_trans;
-               [ apply sequence_mempty with (monoid := BitStringT) |  ]
-               ; idtac "5"
-             | eapply EquivFormat_ComposeIf; intros
-               ; idtac "6"
-             | eapply EquivFormat_trans;
-               [ apply EquivFormat_If_Then_Else with (monoid := BitStringT) |  ]
-               ; idtac "8"
-             | apply EquivFormat_If_Then_Else_Proper
-               ; idtac "9"
-             | eapply EquivFormat_UnderSequence';
-               [ repeat
-                   (eapply EquivFormat_trans;
-                    [ first [eapply EquivFormat_compose_map; idtac "10.0" |
-                              eapply EquivFormat_compose_projection; idtac "10.1" ] |  ] );
-                 apply EquivFormat_reflexive
-               |  ] ; idtac "10"
-             | eapply EquivFormat_Projection_Format_Empty_Format';
-               [ repeat eapply EquivFormat_compose_map;
-                 apply EquivFormat_reflexive ] ; idtac "11"
-             | unfold EquivFormat; intros; reflexivity ]); 
-          intros.
-        normalize_format. 
-        eapply sequence_Compose_format_decode_correct; cycle 1.
-        * unfold format_SumType_list.
-          unfold myFinFormat.
-          (*1*) intros; apply FixList_decode_correct.
-          apply_IndexedSumType_Decoder_Correct 2 types.
-          unfold Vector.nth; simpl; eapply H.
-          simpl;
-            repeat
-              match goal with
-              | |- IterateBoundedIndex.prim_and _ _ =>
-                  apply
-                    IterateBoundedIndex.Build_prim_and
-              end; try exact I; simpl; 
-            intros.
-            3: intros.
-
-          intuition
-              eauto
-              2
-            with data_inv_hints.
-          2: { unfold Vector.nth; simpl; eapply H.
-              | .
-          simpl;
-            repeat
-              match goal with
-              | |- IterateBoundedIndex.prim_and _ _ =>
-                  apply IterateBoundedIndex.Build_prim_and
-              end; try exact I; simpl; intros. ].
+           *)
           
-          apply_rules.
-          
-        * intuition; split; try reflexivity.
-          etransitivity.
-          symmetry; eapply Permutation_length; eauto.
-          simpl; reflexivity.
-          intros ?.
-          match goal with
-          | |-
-              context [ fun st b' =>
-                          ith _ (SumType_index _ st) (SumType_proj _ st) b' ] =>
-                  let a'' := fresh in
-                  intro a''; intros;
-                  repeat instantiate ( 1 := (constant (constant True)) );
-                  repeat destruct a'' as [?| a'']; auto
-          | |-
-              context [ fun st b' =>
-                          ith _ (SumType_index _ st) (SumType_proj _ st) b' ] =>
-                  let a'' := fresh in
-                  intro a''; intros;
-                  repeat instantiate ( 1 := (constant (constant True)) );
-                  repeat destruct a'' as [?| a'']; auto
+          Module PermutationCodes2.  
+        Let types:= [word 8:Type; word 16:Type].
+
+        Let myTuple:= ituple types.
+
+        Definition formats : ilist (B := fun T => FormatM T ByteString) types
+          := {{ format_word; format_word }}.
+        
+        Let invariants := ilist_constant_T types.
+        Let view_fin {n} (f:Fin.t n):= f2n f < pow2 8.
+        Let invariant := (fun st : SumType types =>
+                            view_fin (SumType_index types st) /\ ith invariants (SumType_index types st) (SumType_proj types st)).
+
+        Definition lift_SumType (A:Type) {n:nat} {types:Vector.t Type n} :
+          SumType types -> SumType (Vector.cons Type A _ types):=
+          match types as typs return
+                SumType typs -> SumType (Vector.cons Type A _ typs) with
+          | Vector.nil =>
+              (* Impossible case: with an empty vector can't construct the SumType*)
+              fun elem => let X1 := match elem return A with
+                                    end in X1
+          | Vector.cons a n typs' =>
+              fun elem => inr elem
           end.
-          
-          solve_side_condition.
-          
-          intros; split; auto.
-          admit.
-          shelve.
-        * (*ExtractSource. *)
-          simpl; intros; eapply CorrectDecoderEmpty.
-          -- unfold Heading.Domain, Tuple.GetAttribute, Tuple.GetAttributeRaw,
-               Basics.compose in *; simpl in *.
-               let a' := fresh in
-                intros a'; try destruct a'; destruct_conjs.
-                unfold Heading.Domain, Tuple.GetAttribute, Tuple.GetAttributeRaw in *;
-                  simpl in *; intros. decompose_source_predicate. subst_projections.
-             Require Import Sorting.Sorting.
-             Definition sort: forall A, list A -> list A.
-             Admitted.
+        
+        Fixpoint to_list {n:nat} {S:Type} {types:Vector.t Type n}:
+          forall projections: ilist (B:= fun T => S -> T) types, 
+            S -> list (SumType types):=
+          match types as typs return
+                ilist (B:= fun T => S -> T) typs ->  
+                S -> list (SumType typs) with
+          | Vector.nil => fun _ _ => Datatypes.nil
+          | @Vector.cons _ a n' typs' =>
+              let typs:= Vector.cons Type a n' typs' in
+              fun projs S =>
+                (inj_SumType typs Fin.F1 (prim_fst projs S))
+                  :: map (lift_SumType a) (to_list (prim_snd projs) S)
+          end.
 
-             
-             Definition smart_head {A:Type} (ls: list A): (|ls|) > 0 -> A:=
-               match ls as l return ((| l |) > 0 -> A) with
-               | []%list => fun H : 0 > 0 => ltac:(lia)
-               | a :: ls0 => constant a
-               end.
-             Definition smart_tail {A:Type} (ls: list A): (|ls|) > 0 -> list A:=
-               match ls as l return ((| l |) > 0 -> list A) with
-               | []%list => fun H : 0 > 0 => ltac:(lia)
-               | a :: ls0 => constant ls0
-               end.
+        Definition format_SumType_list
+          (m : nat) (types : Vector.t Type m)
+          (fin_format: FormatM (Fin.t m) ByteString)
+          (formats: ilist (B:= fun T => FormatM T ByteString) types):
+          FormatM (list (SumType types)) ByteString:=
+          format_list (format_IndexedSumType m types formats fin_format).
 
-             Lemma smart_list_split_witness:
-               forall {A ls ls'} {x:A} (H: (x::ls')%list = ls),
-                 (|ls|) > 0.
-             Proof.
-               intros. destruct ls; simpl in *; try discriminate.
-               unfold ">".
-               lia.
-             Qed.
-             Lemma smart_list_split:
-               forall A ls ls' (x:A) (H: (x::ls')%list = ls),
-                 x = smart_head ls (smart_list_split_witness H) /\
-                   ls' = smart_tail ls (smart_list_split_witness H).
-             Proof. intros; split; subst ls; reflexivity. Qed.
-             
-             
-             Instance Permutation_ConditionallyInvertibleRel {n}{types: Vector.t Type n}:
-                      ConditionallyInvertibleRel (@Permutation (SumType types))
-                      (fun a => Sorted eq a) (sort (SumType types)).
-             Proof.
-               constructor.
-               intros.
-             Admitted.
+        
+        Definition format_permutation_list
+          (m : nat) (types : Vector.t Type m)
+          (fin_format: FormatM (Fin.t m) ByteString)
+          (formats: ilist (B:= fun T => FormatM T ByteString) types):
+          FormatM (list (SumType types)) ByteString:=
+          Compose_Format (format_SumType_list m types fin_format formats)
+            (Permutation (A:=SumType types)).
+        
+        
+        
+        Definition format_through_list
+          S
+          (m : nat) (types : t Type m)
+          (projections: ilist (B:= fun T => S -> T) types)
+          (fin_format: FormatM (Fin.t m) ByteString)
+          (formats: ilist (B:= fun T => FormatM T ByteString) types):
+          FormatM S ByteString:=
+          format_permutation_list m types fin_format formats ◦ to_list projections.
+        
+        Record message := {
+            label : word 8
+          ; data : word 16                     
+          }.
 
-             Print Instances ConditionallyInvertibleRel.
-             eapply CInvRoundTripRel in H0.
-             Ltac blah:= match goal with
-                         | [H: (?a::?ls')%list = ?x |- _ ] =>
-                             let HH:= fresh "HH" in
-                             idtac H;
-                             pose proof (smart_list_split _ _ _ _ H) as HH;
-                             try clear H; destruct HH
-                         end.
-             blah.
-             blah.
-             Definition inv_inr: (
-             clear H0.
-             
-             
-             
-             2: { admit. }
+        Let myProjections: ilist (B:=fun T => _ -> T) types := {{ label ; data }}.
+        Let myTypes {n: nat} {types: Vector.t Type n} {B} (list: ilist (B:=B) types): Vector.t Type n:= types.
+        
+        Let myCodes: Vector.t (word 8) 2:= [[ natToWord _ 42; natToWord _ 73 ]].
+        Let myFinFormat:= (format_enum myCodes).
+        
+        Let myFormats: ilist (B := fun T => FormatM T ByteString) (myTypes myProjections) := {{ format_word; format_word }}.
+        
+        Let myFormat:= format_through_list message _ types myProjections myFinFormat myFormats.
+        
+        Let enc_dec : EncoderDecoderPair myFormat (constant True).
+        Proof.
+          (*unfold myFormat,format_through_list, format_permutation_list.*)
+          (* derive_encoder_decoder_pair. *)
+          econstructor.
+          - (* synthesize_aligned_encoder. *)
+            start_synthesizing_encoder.
+            normalize_encoder_format.
+            
+            align_encoder_step. (*splits emty*)
+            align_encoder_step. (* removes empty*)
+            (*eapply CorrectAlignedEncoderProjection.*)
+            align_encoder_step. (*projection*)
+            
+            unfold format_permutation_list.
+            match goal with
+              |- CorrectAlignedEncoder (Compose_Format ?X _) ?enc =>
+                cut (CorrectAlignedEncoder X enc) 
+            end.
+            + (*This should be trivial, since identity is a premutation*)
+              unfold format_SumType_list.
+              shelve.
+            + repeat align_encoder_step.
+          - (* synthesize_aligned_decoder. *)
+            start_synthesizing_decoder.
+            + Lemma EquivFormat_compose_projection {T S S' S''}
+                (format_S'' : FormatM S'' T)
+                (f : S -> S')
+                (r : S' -> S'' -> Prop)
+                : EquivFormat (Projection_Format (Compose_Format format_S'' r) f)
+                    (Compose_Format format_S'' (fun a b => r (f a) b)).
+              Proof.
+                unfold EquivFormat, refineEquiv, Projection_Format, Compose_Format, compose, Bind2; split;
+                  intros ? ?.
+                - rewrite unfold_computes in *.
+                  destruct_ex; split_and; eexists.
+                  rewrite unfold_computes;  eauto.
+                - rewrite unfold_computes in *.
+                  destruct_ex; split_and.
+                  rewrite unfold_computes in H0.
+                  destruct_ex; split_and.
+                  eexists; intuition eauto.
+                  subst; eauto.
+              Qed.
 
-             Ltac blah:=
-               match goal with
-               | [H: (?a::?ls')%list = ?x |- _ ] => 
-                   let HH:= fresh "HH" in
-                   destruct x eqn:HH; try discriminate;
-                   injection H; try clear H;
-                   let H':=fresh in
-                   let Hnew_eq:= fresh "Hnew_eq" in
-                   intros H' Hnew_eq
-               | [H: ([])%list = ?x |- _ ] =>
-                   subst x
-               end.
+              Ltac normalize_step BitStringT ::=
+                (first_debug
+                   [ match goal with
+                     | |- EquivFormat ?z ?x => is_evar z; apply EquivFormat_reflexive
+                     end; idtac "1"
+                   | eapply EquivFormat_trans; [ apply sequence_assoc |  ]
+                     ; idtac "3"
+                   | eapply EquivFormat_trans;
+                     [ apply sequence_mempty with (monoid := BitStringT) |  ]
+                     ; idtac "5"
+                   | eapply EquivFormat_ComposeIf; intros
+                     ; idtac "6"
+                   | eapply EquivFormat_trans;
+                     [ apply EquivFormat_If_Then_Else with (monoid := BitStringT) |  ]
+                     ; idtac "8"
+                   | apply EquivFormat_If_Then_Else_Proper
+                     ; idtac "9"
+                   | eapply EquivFormat_UnderSequence';
+                     [ repeat
+                         (eapply EquivFormat_trans;
+                          [ first [eapply EquivFormat_compose_map; idtac "10.0" |
+                                    eapply EquivFormat_compose_projection; idtac "10.1" ] |  ] );
+                       apply EquivFormat_reflexive
+                     |  ] ; idtac "10"
+                   | eapply EquivFormat_Projection_Format_Empty_Format';
+                     [ repeat eapply EquivFormat_compose_map;
+                       apply EquivFormat_reflexive ] ; idtac "11"
+                   | unfold EquivFormat; intros; reflexivity ]); 
+                intros.
+              normalize_format. 
+              eapply sequence_Compose_format_decode_correct; cycle 1.
+              * unfold format_SumType_list.
+                unfold myFinFormat.
+                (*1*) intros; apply FixList_decode_correct.
+                apply_IndexedSumType_Decoder_Correct 2 types.
+                unfold Vector.nth; simpl; eapply H.
+                simpl;
+                  repeat
+                    match goal with
+                    | |- IterateBoundedIndex.prim_and _ _ =>
+                        apply
+                          IterateBoundedIndex.Build_prim_and
+                    end; try exact I; simpl; 
+                  intros.
+                3: intros.
 
-             repeat blah.
-             
+                intuition
+                  eauto
+                    2
+                  with data_inv_hints.
+                2: { unfold Vector.nth; simpl; eapply H.
+                     | .
+                     simpl;
+                       repeat
+                         match goal with
+                         | |- IterateBoundedIndex.prim_and _ _ =>
+                             apply IterateBoundedIndex.Build_prim_and
+                         end; try exact I; simpl; intros. ].
+                
+                apply_rules.
+                
+              * intuition; split; try reflexivity.
+                etransitivity.
+                symmetry; eapply Permutation_length; eauto.
+                simpl; reflexivity.
+                intros ?.
+                match goal with
+                | |-
+                    context [ fun st b' =>
+                                ith _ (SumType_index _ st) (SumType_proj _ st) b' ] =>
+                    let a'' := fresh in
+                    intro a''; intros;
+                    repeat instantiate ( 1 := (constant (constant True)) );
+                    repeat destruct a'' as [?| a'']; auto
+                | |-
+                    context [ fun st b' =>
+                                ith _ (SumType_index _ st) (SumType_proj _ st) b' ] =>
+                    let a'' := fresh in
+                    intro a''; intros;
+                    repeat instantiate ( 1 := (constant (constant True)) );
+                    repeat destruct a'' as [?| a'']; auto
+                end.
+                
+                solve_side_condition.
+                
+                intros; split; auto.
+                admit.
+                shelve.
+              * (*ExtractSource. *)
+                simpl; intros; eapply CorrectDecoderEmpty.
+                -- unfold Heading.Domain, Tuple.GetAttribute, Tuple.GetAttributeRaw,
+                     Basics.compose in *; simpl in *.
+                   let a' := fresh in
+                   intros a'; try destruct a'; destruct_conjs.
+                   unfold Heading.Domain, Tuple.GetAttribute, Tuple.GetAttributeRaw in *;
+                     simpl in *; intros. decompose_source_predicate. subst_projections.
+                   Require Import Sorting.Sorting.
+                   Definition sort: forall A, list A -> list A.
+                   Admitted.
 
-             unshelve instantiate(1:=_).
-             
-             
-               
-               match goal with
-               | H:?f ?x ?y
-                 |- _ =>
-                   eapply CInvRoundTripRel in H;
-                   [  | now typeclasses eauto | now simpl in *; eauto ]; 
-                   try subst x
-               end.
-               
-               Lemma Permutation_remove
+                   
+                   Definition smart_head {A:Type} (ls: list A): (|ls|) > 0 -> A:=
+                     match ls as l return ((| l |) > 0 -> A) with
+                     | []%list => fun H : 0 > 0 => ltac:(lia)
+                     | a :: ls0 => constant a
+                     end.
+                   Definition smart_tail {A:Type} (ls: list A): (|ls|) > 0 -> list A:=
+                     match ls as l return ((| l |) > 0 -> list A) with
+                     | []%list => fun H : 0 > 0 => ltac:(lia)
+                     | a :: ls0 => constant ls0
+                     end.
+
+                   Lemma smart_list_split_witness:
+                     forall {A ls ls'} {x:A} (H: (x::ls')%list = ls),
+                       (|ls|) > 0.
+                   Proof.
+                     intros. destruct ls; simpl in *; try discriminate.
+                     unfold ">".
+                     lia.
+                   Qed.
+                   Lemma smart_list_split:
+                     forall A ls ls' (x:A) (H: (x::ls')%list = ls),
+                       x = smart_head ls (smart_list_split_witness H) /\
+                         ls' = smart_tail ls (smart_list_split_witness H).
+                   Proof. intros; split; subst ls; reflexivity. Qed.
+                   
+                   
+                   Instance Permutation_ConditionallyInvertibleRel {n}{types: Vector.t Type n}:
+                     ConditionallyInvertibleRel (@Permutation (SumType types))
+                       (fun a => Sorted eq a) (sort (SumType types)).
+                   Proof.
+                     constructor.
+                     intros.
+                   Admitted.
+
+                   Print Instances ConditionallyInvertibleRel.
+                   eapply CInvRoundTripRel in H0.
+                   Ltac blah:= match goal with
+                               | [H: (?a::?ls')%list = ?x |- _ ] =>
+                                   let HH:= fresh "HH" in
+                                   idtac H;
+                                   pose proof (smart_list_split _ _ _ _ H) as HH;
+                                   try clear H; destruct HH
+                               end.
+                   blah.
+                   blah.
+                   Definition inv_inr: (
+                                         clear H0.
                      
                      
-                 subst_invertible. reflexivity).
+                     
+                     2: { admit. }
+
+                     Ltac blah:=
+                       match goal with
+                       | [H: (?a::?ls')%list = ?x |- _ ] => 
+                           let HH:= fresh "HH" in
+                           destruct x eqn:HH; try discriminate;
+                           injection H; try clear H;
+                           let H':=fresh in
+                           let Hnew_eq:= fresh "Hnew_eq" in
+                           intros H' Hnew_eq
+                       | [H: ([])%list = ?x |- _ ] =>
+                           subst x
+                       end.
+
+                     repeat blah.
+                     
+
+                     unshelve instantiate(1:=_).
+                     
+                     
+                     
+                     match goal with
+                     | H:?f ?x ?y
+                       |- _ =>
+                         eapply CInvRoundTripRel in H;
+                         [  | now typeclasses eauto | now simpl in *; eauto ]; 
+                         try subst x
+                     end.
+                     
+                     Lemma Permutation_remove
+                             
+                             
+                       subst_invertible. reflexivity).
 
 
-                                               | decide_data_invariant ] ].
+                   | decide_data_invariant ] ].
 
-                                                                          
-                                                                          
-                                                                          lazymatch goal with
-                                                                            |- CorrectDecoder ?mon _ _ _ (Compose_Format ?YY ?R ++ _) _ _ _ =>
-                                                                              remember YY as XX
-                                                                          end.
-                                                                          exploit @sequence_Compose_format_decode_correct.
-                                                                          5:{ intros HH.
-                                                                              match type of HH with
-                                                                                CorrectDecoder ByteStringQueueMonoid ?Goal11 
-                                                                                               ?Goal11 eq (Compose_Format ?Goal13 ?Goal10 ++ ?Goal14)
-                                                                                               (sequence_Decode ?Goal15 ?Goal18) ?Goal6
-                             (Compose_Format ?Goal13 ?Goal10 ++ ?Goal14) =>
-                unify Goal11 ((fun _ : message => True));
-                try unify Goal13 XX;
-                unify Goal10 (fun (a' : message) (b' : list (SumType types)) =>
-                                Permutation [inl (label a'); inr (data a')] b') 
-            end.
-            revert HH.
-            lazymatch goal with
-              |- CorrectDecoder ByteStringQueueMonoid (constant True) 
-                               (constant True) eq
-                               (Compose_Format XX
-                                               (fun (a' : message) (b' : list (SumType types)) =>
-                                                  Permutation [inl (label a'); inr (data a')] b') ++ 
-                                               ?Goal9) ?Goal10 ?Goal4
-                               (Compose_Format XX
-                                               (fun (a' : message) (b' : list (SumType types)) =>
-                                                  Permutation [inl (label a'); inr (data a')] b') ++ 
-                                               ?Goal9) ->
-                CorrectDecoder AlignedByteString.ByteStringQueueMonoid 
-                               (constant True) (constant True) eq
-                               (Compose_Format XX
-                                               (fun (a' : message) (b' : list (SumType types)) =>
-                                                  Permutation [inl (label a'); inr (data a')] b') ++ ?empty_Format)
-                               ?decoder ?cache_inv
-                               (Compose_Format XX
-                                               (fun (a' : message) (b' : list (SumType types)) =>
-                                                  Permutation [inl (label a'); inr (data a')] b')) =>
-                unify decoder Goal10;
-                unify cache_inv Goal4
-            end.
-            unshelve instantiate(4:=_). eapply empty_Format.
-            intros HH. eapply HH.
-            
-            eapply HH.
-            unshelve instantiate(2:= _) in HH.
-            
-            eapply HH.
-        unfold "◦".
-        eapply (format_sequence_correct H) with (monoid :=  AlignedByteString.ByteStringQueueMonoid ).
-        * clear H; intros; apply_rules.
-          
-          exploit @Compose_decode_correct.
-          3: { intros HH.
-               match type of HH with
-                 CorrectDecoder ?mon ?g9 ?g10 ?g8 (Compose_Format ?g11 ?g8) ?g13 ?g7 ?g12 =>
-                   unify g9 g10;
-                   unify g8 eq;
-                   unify g11
-               end.
-            
-          
-        * clear H. (*solve [ solve_side_condition ].*) shelve.
-        * clear H; intros; apply_rules.
+                                              
+                                              
+                                              lazymatch goal with
+                                                |- CorrectDecoder ?mon _ _ _ (Compose_Format ?YY ?R ++ _) _ _ _ =>
+                                                  remember YY as XX
+                                              end.
+                                              exploit @sequence_Compose_format_decode_correct.
+                                              5:{ intros HH.
+                                                  match type of HH with
+                                                    CorrectDecoder ByteStringQueueMonoid ?Goal11 
+                                                      ?Goal11 eq (Compose_Format ?Goal13 ?Goal10 ++ ?Goal14)
+                                                      (sequence_Decode ?Goal15 ?Goal18) ?Goal6
+                                                      (Compose_Format ?Goal13 ?Goal10 ++ ?Goal14) =>
+                                                      unify Goal11 ((fun _ : message => True));
+                                                      try unify Goal13 XX;
+                                                      unify Goal10 (fun (a' : message) (b' : list (SumType types)) =>
+                                                                      Permutation [inl (label a'); inr (data a')] b') 
+                                                  end.
+                                                  revert HH.
+                                                  lazymatch goal with
+                                                    |- CorrectDecoder ByteStringQueueMonoid (constant True) 
+                                                         (constant True) eq
+                                                         (Compose_Format XX
+                                                            (fun (a' : message) (b' : list (SumType types)) =>
+                                                               Permutation [inl (label a'); inr (data a')] b') ++ 
+                                                            ?Goal9) ?Goal10 ?Goal4
+                                                         (Compose_Format XX
+                                                            (fun (a' : message) (b' : list (SumType types)) =>
+                                                               Permutation [inl (label a'); inr (data a')] b') ++ 
+                                                            ?Goal9) ->
+                                                       CorrectDecoder AlignedByteString.ByteStringQueueMonoid 
+                                                         (constant True) (constant True) eq
+                                                         (Compose_Format XX
+                                                            (fun (a' : message) (b' : list (SumType types)) =>
+                                                               Permutation [inl (label a'); inr (data a')] b') ++ ?empty_Format)
+                                                         ?decoder ?cache_inv
+                                                         (Compose_Format XX
+                                                            (fun (a' : message) (b' : list (SumType types)) =>
+                                                               Permutation [inl (label a'); inr (data a')] b')) =>
+                                                      unify decoder Goal10;
+                                                      unify cache_inv Goal4
+                                                  end.
+                                                  unshelve instantiate(4:=_). eapply empty_Format.
+                                                  intros HH. eapply HH.
+                                                  
+                                                  eapply HH.
+                                                  unshelve instantiate(2:= _) in HH.
+                                                  
+                                                  eapply HH.
+                                                  unfold "◦".
+                                                  eapply (format_sequence_correct H) with (monoid :=  AlignedByteString.ByteStringQueueMonoid ).
+                                                  * clear H; intros; apply_rules.
+                                                    
+                                                    exploit @Compose_decode_correct.
+                                                    3: { intros HH.
+                                                         match type of HH with
+                                                           CorrectDecoder ?mon ?g9 ?g10 ?g8 (Compose_Format ?g11 ?g8) ?g13 ?g7 ?g12 =>
+                                                             unify g9 g10;
+                                                             unify g8 eq;
+                                                             unify g11
+                                                         end.
+                                                         
+                                                         
+                                                         * clear H. (*solve [ solve_side_condition ].*) shelve.
+                                                         * clear H; intros; apply_rules.
 
-        apply_rules.
-      + cbv beta; synthesize_cache_invariant.
-      + cbv beta; unfold decode_nat, sequence_Decode; optimize_decoder_impl.
-      + cbv beta; align_decoders.
-      
+                                                           apply_rules.
+                                                         + cbv beta; synthesize_cache_invariant.
+                                                         + cbv beta; unfold decode_nat, sequence_Decode; optimize_decoder_impl.
+                                                         + cbv beta; align_decoders.
+                                                           
 
-    
-    Unshelve.
-    (* This one is due to way `align_decoders_step`  deals with
+                                                           
+                                                           Unshelve.
+                                                           (* This one is due to way `align_decoders_step`  deals with
        `IterateBoundedIndex.prim_and`.
        There is an already shelved `ilist` that slowly
        decreases but obviously never gets completed (since the last goal doesn't depend).
-     *)
-    constructor.
-  Defined.
-        
-  Let encode := encoder_impl enc_dec.
-  
-  Let decode := decoder_impl enc_dec.
-    Print Assumptions decode.
-    
-End SumTypeCodes2.
+                                                            *)
+                                                           constructor.
+                                              Defined.
+                                              
+                                              Let encode := encoder_impl enc_dec.
+                                              
+                                              Let decode := decoder_impl enc_dec.
+                                              Print Assumptions decode.
+                                              
+                                              End SumTypeCodes2.
 
-(** * Repeated type*)
-(* | In this module show that IndexedSumType, by virtue of using an index, supports repeated types.
+                                              (** * Repeated type*)
+                                              (* | In this module show that IndexedSumType, by virtue of using an index, supports repeated types.
    Here the `word 8` type is repeated but, depending on the index, it will use the first or third format.
 
    We are still using words to directly encode indices
- *)
+                                               *)
 
-Module SumTypeCodes3.
+                                              Module SumTypeCodes3.
 
-    Let types:= [word 8:Type; word 16:Type; word 8:Type].
-    Definition formats : ilist (B := fun T => FormatM T ByteString) types
-    := {{ format_word; format_word ; format_word }}.
+                                                Let types:= [word 8:Type; word 16:Type; word 8:Type].
+                                                Definition formats : ilist (B := fun T => FormatM T ByteString) types
+                                                  := {{ format_word; format_word ; format_word }}.
 
-    Let invariants := ilist_constant_T types.
-    
-    Let view_fin {n} (f:Fin.t n):= f2n f < pow2 8.
+                                                Let invariants := ilist_constant_T types.
+                                                
+                                                Let view_fin {n} (f:Fin.t n):= f2n f < pow2 8.
 
-    Let invariant := (fun st : SumType types =>
-                        view_fin (SumType_index types st) /\ ith invariants (SumType_index types st) (SumType_proj types st)).
-        
-    Let enc_dec : EncoderDecoderPair (format_IndexedSumType_word 8 formats) invariant.
-    Proof.
-      unfold format_IndexedSumType_word.
-      derive_encoder_decoder_pair.
-      
-      (* (*below are the instructions to do the automation step-by-step*)
+                                                Let invariant := (fun st : SumType types =>
+                                                                    view_fin (SumType_index types st) /\ ith invariants (SumType_index types st) (SumType_proj types st)).
+                                                
+                                                Let enc_dec : EncoderDecoderPair (format_IndexedSumType_word 8 formats) invariant.
+                                                Proof.
+                                                  unfold format_IndexedSumType_word.
+                                                  derive_encoder_decoder_pair.
+                                                  
+                                                  (* (*below are the instructions to do the automation step-by-step*)
 
       econstructor.
       - synthesize_aligned_encoder.
@@ -861,111 +731,111 @@ Module SumTypeCodes3.
         + cbv beta; unfold decode_nat, sequence_Decode; optimize_decoder_impl.
         + cbv beta.
           repeat align_decoders_step. *)
-          
+                                                  
 
-      
-      (* align_decoders_step' *)
-      (* AlignedDecodeSumTypeM *)
-      
-      Unshelve.
-        (* This one is due to way `align_decoders_step`  deals with
+                                                  
+                                                  (* align_decoders_step' *)
+                                                  (* AlignedDecodeSumTypeM *)
+                                                  
+                                                  Unshelve.
+                                                  (* This one is due to way `align_decoders_step`  deals with
            `IterateBoundedIndex.prim_and`.
            There is an already shelved `ilist` that slowly
            decreases but obviously never gets completed (since the last goal doesn't depend).
-         *)
-        constructor.
-    Defined.
-        
-  Let encode := encoder_impl enc_dec.
-  
-  Let decode := decoder_impl enc_dec.
-    Print Assumptions decode.
-    
-End SumTypeCodes3.
+                                                   *)
+                                                  constructor.
+                                                Defined.
+                                                
+                                                Let encode := encoder_impl enc_dec.
+                                                
+                                                Let decode := decoder_impl enc_dec.
+                                                Print Assumptions decode.
+                                                
+                                              End SumTypeCodes3.
 
 
-(** * Simple indexed sumtype (two formats)*)
-(* | In this module we show different ways to encode the index.  Here
+                                              (** * Simple indexed sumtype (two formats)*)
+                                              (* | In this module we show different ways to encode the index.  Here
    the index is encoded by a word (representing a label) which is
    looked up in a vector to determine the index.
- *)
-Module SumTypeCodes_Enum.
-  
-  Let types:= [word 8:Type; word 16:Type].
-  
-  Definition formats : ilist (B := fun T => FormatM T ByteString) types
-    := {{ format_word; format_word }}.
-  
-  Let invariants := ilist_constant_T types.
-  Let view_fin {n} (f:Fin.t n):= f2n f < pow2 8.
-  Let constT {T} (a:T):= True.
-  Let invariant := (fun st : SumType types =>  ((constant True) (SumType_index types st)) /\ ith invariants (SumType_index types st) (SumType_proj types st)).
-  
-  Let codes: Vector.t (word 8) 2:= [[ natToWord _ 42; natToWord _ 73 ]].
-        
-  Let enc_dec : EncoderDecoderPair (format_IndexedSumType_enum _ codes formats) invariant.
-  Proof.
-    unfold format_IndexedSumType_enum.
-    derive_encoder_decoder_pair.
+                                               *)
+                                              Module SumTypeCodes_Enum.
+                                                
+                                                Let types:= [word 8:Type; word 16:Type].
+                                                
+                                                Definition formats : ilist (B := fun T => FormatM T ByteString) types
+                                                  := {{ format_word; format_word }}.
+                                                
+                                                Let invariants := ilist_constant_T types.
+                                                Let view_fin {n} (f:Fin.t n):= f2n f < pow2 8.
+                                                Let constT {T} (a:T):= True.
+                                                Let invariant := (fun st : SumType types =>  ((constant True) (SumType_index types st)) /\ ith invariants (SumType_index types st) (SumType_proj types st)).
+                                                
+                                                Let codes: Vector.t (word 8) 2:= [[ natToWord _ 42; natToWord _ 73 ]].
+                                                
+                                                Let enc_dec : EncoderDecoderPair (format_IndexedSumType_enum _ codes formats) invariant.
+                                                Proof.
+                                                  unfold format_IndexedSumType_enum.
+                                                  derive_encoder_decoder_pair.
 
-      Unshelve.
-        (* This one is due to way `align_decoders_step`  deals with
+                                                  Unshelve.
+                                                  (* This one is due to way `align_decoders_step`  deals with
            `IterateBoundedIndex.prim_and`.
            There is an already shelved `ilist` that slowly
            decreases but obviously never gets completed (since the last goal doesn't depend).
-         *)
-    constructor.
-  Defined.
-  
-  Let encode := encoder_impl enc_dec.
-  
-  Let decode := decoder_impl enc_dec.
-  
-End SumTypeCodes_Enum.
+                                                   *)
+                                                  constructor.
+                                                Defined.
+                                                
+                                                Let encode := encoder_impl enc_dec.
+                                                
+                                                Let decode := decoder_impl enc_dec.
+                                                
+                                              End SumTypeCodes_Enum.
 
 
-(** * Motivating example*)
-(* | Another example using Enum, which originally motivated this format.
- *)
-Module SumTypeCodes_Enum_Motivate.
+                                              (** * Motivating example*)
+                                              (* | Another example using Enum, which originally motivated this format.
+                                               *)
+                                              Module SumTypeCodes_Enum_Motivate.
 
-  (* This was the motivating example, which follows immidiately from out `format_IndexedSumType_enum` *)
-  Definition format_SumTypeCodes {m} {sz}
-             (types : Vector.t Type (S m))
-             (formatrs :
-                ilist (B := fun T =>
-                 T -> CacheFormat -> Comp (ByteString * CacheFormat)) types)
-             (codes : Vector.t (word sz) (S m))
-             (st : SumType types)
-    : CacheFormat -> Comp (ByteString * CacheFormat):=
-    format_IndexedSumType_enum m codes formatrs st.
+                                                (* This was the motivating example, which follows immidiately from out `format_IndexedSumType_enum` *)
+                                                Definition format_SumTypeCodes {m} {sz}
+                                                  (types : Vector.t Type (S m))
+                                                  (formatrs :
+                                                    ilist (B := fun T =>
+                                                                  T -> CacheFormat -> Comp (ByteString * CacheFormat)) types)
+                                                  (codes : Vector.t (word sz) (S m))
+                                                  (st : SumType types)
+                                                  : CacheFormat -> Comp (ByteString * CacheFormat):=
+                                                  format_IndexedSumType_enum m codes formatrs st.
 
-  (* Then we can show an example with that format *)
-  Let types:= [word 8:Type; word 16:Type; word 32:Type; word 16:Type; word 8:Type].
-  
-  Definition formats : ilist (B := fun T => FormatM T ByteString) types
-    := {{ format_word; format_word; format_word; format_word; format_word }}.
-  
-  Let invariants := ilist_constant_T types.
-  Let view_fin {n} (f:Fin.t n):= f2n f < pow2 8.
-  Let constT {T} (a:T):= True.
-  Let invariant := (fun st : SumType types =>  ((constant True) (SumType_index types st)) /\ ith invariants (SumType_index types st) (SumType_proj types st)).
+                                                (* Then we can show an example with that format *)
+                                                Let types:= [word 8:Type; word 16:Type; word 32:Type; word 16:Type; word 8:Type].
+                                                
+                                                Definition formats : ilist (B := fun T => FormatM T ByteString) types
+                                                  := {{ format_word; format_word; format_word; format_word; format_word }}.
+                                                
+                                                Let invariants := ilist_constant_T types.
+                                                Let view_fin {n} (f:Fin.t n):= f2n f < pow2 8.
+                                                Let constT {T} (a:T):= True.
+                                                Let invariant := (fun st : SumType types =>  ((constant True) (SumType_index types st)) /\ ith invariants (SumType_index types st) (SumType_proj types st)).
 
-  (* Let's index the entries using prime numbers *)
-  Let codes: Vector.t (word 8) 5:= [[ natToWord _ 2; natToWord _ 3; natToWord _ 5; natToWord _ 7; natToWord _ 11 ]].
+                                                (* Let's index the entries using prime numbers *)
+                                                Let codes: Vector.t (word 8) 5:= [[ natToWord _ 2; natToWord _ 3; natToWord _ 5; natToWord _ 7; natToWord _ 11 ]].
 
-  Let enc_dec : EncoderDecoderPair (format_SumTypeCodes types formats codes) invariant.
-  Proof.
-    unfold format_SumTypeCodes, format_IndexedSumType_enum.
-    derive_encoder_decoder_pair.
+                                                Let enc_dec : EncoderDecoderPair (format_SumTypeCodes types formats codes) invariant.
+                                                Proof.
+                                                  unfold format_SumTypeCodes, format_IndexedSumType_enum.
+                                                  derive_encoder_decoder_pair.
 
-      Unshelve.
-        (* This one is due to way `align_decoders_step`  deals with
+                                                  Unshelve.
+                                                  (* This one is due to way `align_decoders_step`  deals with
            `IterateBoundedIndex.prim_and`.
            There is an already shelved `ilist` that slowly
            decreases but obviously never gets completed (since the last goal doesn't depend).
-         *)
-    constructor.
-  Defined.
-  
-End SumTypeCodes_Enum_Motivate.
+                                                   *)
+                                                  constructor.
+                                                Defined.
+                                                
+                                              End SumTypeCodes_Enum_Motivate.
